Source/DafnyCore/Compilers/Cplusplus/Compiler-cpp.cs
@@ -1506,24 +1506,24 @@ namespace Microsoft.Dafny.Compilers {
       return s;
     }
 
-    protected override ConcreteSyntaxTree EmitBitvectorTruncation(BitvectorType bvType, bool surroundByUnchecked, ConcreteSyntaxTree wr) {
-      string nativeName = null, literalSuffix = null;
-      bool needsCastAfterArithmetic = false;
-      if (bvType.NativeType != null) {
-        GetNativeInfo(bvType.NativeType.Sel, out nativeName, out literalSuffix, out needsCastAfterArithmetic);
+    protected override ConcreteSyntaxTree EmitBitvectorTruncation(BitvectorType bvType, [CanBeNull] NativeType nativeType,
+      bool surroundByUnchecked, ConcreteSyntaxTree wr) {
+      string literalSuffix = null;
+      if (nativeType != null) {
+        GetNativeInfo(nativeType.Sel, out _, out literalSuffix, out _);
       }
 
-      if (bvType.NativeType == null) {
+      if (nativeType == null) {
         throw new UnsupportedFeatureException(Token.NoToken, Feature.UnboundedIntegers, "EmitBitvectorTruncation with BigInteger value");
-      } else if (bvType.NativeType.Bitwidth == bvType.Width) {
-        // no truncation needed
-        return wr;
-      } else {
+      } else if (bvType.Width < nativeType.Bitwidth) {
         wr.Write("((");
         var middle = wr.Fork();
         // print in hex, because that looks nice
         wr.Write(") & 0x{0:X}{1})", (1UL << bvType.Width) - 1, literalSuffix);
         return middle;
+      } else {
+        // no truncation needed
+        return wr;
       }
     }
 
@@ -2135,7 +2135,7 @@ namespace Microsoft.Dafny.Compilers {
           opString = ">";
           break;
         case BinaryExpr.ResolvedOpcode.LeftShift:
-          if (resultType.IsBitVectorType) {
+          if (resultType.NormalizeToAncestorType().IsBitVectorType) {
             truncateResult = true;
           }
           if (AsNativeType(resultType) != null) {
@@ -2157,7 +2157,7 @@ namespace Microsoft.Dafny.Compilers {
           }
           break;
         case BinaryExpr.ResolvedOpcode.Add:
-          if (resultType.IsBitVectorType) {
+          if (resultType.NormalizeToAncestorType().IsBitVectorType) {
             truncateResult = true;
           }
           if (resultType.IsCharType || AsNativeType(resultType) != null) {
@@ -2168,7 +2168,7 @@ namespace Microsoft.Dafny.Compilers {
           }
           break;
         case BinaryExpr.ResolvedOpcode.Sub:
-          if (resultType.IsBitVectorType) {
+          if (resultType.NormalizeToAncestorType().IsBitVectorType) {
             truncateResult = true;
           }
           if (resultType.IsCharType || AsNativeType(resultType) != null) {
@@ -2178,7 +2178,7 @@ namespace Microsoft.Dafny.Compilers {
           }
           break;
         case BinaryExpr.ResolvedOpcode.Mul:
-          if (resultType.IsBitVectorType) {
+          if (resultType.NormalizeToAncestorType().IsBitVectorType) {
             truncateResult = true;
           }
           if (AsNativeType(resultType) != null) {
