Source/DafnyCore/Compilers/Dafny/Compiler-dafny.cs
@@ -1267,7 +1267,8 @@ namespace Microsoft.Dafny.Compilers {
       throw new InvalidOperationException();
     }
 
-    protected override ConcreteSyntaxTree EmitBitvectorTruncation(BitvectorType bvType, bool surroundByUnchecked, ConcreteSyntaxTree wr) {
+    protected override ConcreteSyntaxTree EmitBitvectorTruncation(BitvectorType bvType, [CanBeNull] NativeType nativeType,
+      bool surroundByUnchecked, ConcreteSyntaxTree wr) {
       throwGeneralUnsupported();
       throw new InvalidOperationException();
     }
