Source/DafnyRuntime/DafnyRuntime.cs
@@ -1656,17 +1656,17 @@ namespace Dafny {
     }
 
     public static uint Bv32ShiftLeft(uint a, int amount) {
-      return amount == 32 ? 0 : a << amount;
+      return 32 <= amount ? 0 : a << amount;
     }
     public static ulong Bv64ShiftLeft(ulong a, int amount) {
-      return amount == 64 ? 0 : a << amount;
+      return 64 <= amount ? 0 : a << amount;
     }
 
     public static uint Bv32ShiftRight(uint a, int amount) {
-      return amount == 32 ? 0 : a >> amount;
+      return 32 <= amount ? 0 : a >> amount;
     }
     public static ulong Bv64ShiftRight(ulong a, int amount) {
-      return amount == 64 ? 0 : a >> amount;
+      return 64 <= amount ? 0 : a >> amount;
     }
   }
 
