Source/IntegrationTests/TestFiles/LitTests/LitTest/comp/GeneralNewtypes.dfy
@@ -7,6 +7,7 @@ method Main() {
   BaseTypesThatAreSubsetTypes.Test();
   TypeDescriptors.Test();
   PrintChars.Test();
+  Bitvectors.Test();
 }
 
 module Numerics {
@@ -289,5 +290,204 @@ module PrintChars {
 
   method Print<X, Y>(x: X, y: Y) {
     print x, " ", y, "\n"; // 'c' 'm'
+  }
+}
+
+module Bitvectors {
+  newtype BV = b: bv5 | b != 23
+  newtype Word = bv32
+  newtype Big = b: bv1024 | true
+  newtype int32 = x: int | -0x8000_0000 <= x < 0x8000_0000
+  newtype MyReal = r: real | true
+
+  datatype Color = Blue | Yellow
+  trait RefTrait extends object { }
+  class MyClass extends RefTrait { }
+
+  type Subset = b: bv5 | b != 23
+
+  method Test() {
+    IntermediateExpressions();
+    var _, _ := Operations(7, 0x1234_abcd, -6);
+    Overflows();
+    var _ := Shift(18, 1, 2, 3);
+    var _, _ := Rotate(18, 2, 2, 3);
+    BvZero(0);
+    var _, _, _, _, _, _, _, _, _ := TestsAndConversions();
+
+    var size := Comprehensions({9, 11}, {3}, {200, 190, 191}, {17} + {18});
+    print size, "\n"; // 8
+  }
+
+  method IntermediateExpressions() {
+    var fem: bv5 := 5;
+    var sju: Subset := 4 + 3;
+    var nio: BV := 1 + 8;
+
+    assert fem == 5 && sju == 7 && nio == 9;
+    print fem, sju, nio, "\n"; // 579
+  }
+
+  method Operations(x: BV, y: Word, z: Big) returns (r: bool, s: BV) {
+    // ==
+    r := x == x;
+    r := y == y;
+    r := z == z;
+
+    r := x == 5;
+
+    // + - * / %
+    if x != 0 {
+      s := x + x - x * (x / x - x % x);
+      print s, " ";
+    }
+    if 3 <= x < 8 {
+      s := 12 + x - (x + 19 / 17 - x % 3);
+      print s, " ";
+    }
+    s := 12 + 13 - 14 * (15 + 16 / 17 - 18 % 19);
+    print s, " ";
+
+    // & | ^
+    s := (x & x) | (x ^ x ^ x);
+    print s, " "; // 7
+    s := (12 & 13) | (14 ^ 15 ^ 16);
+    print s, " ";
+
+    // < <= >= >
+    r := (x <= x && x < x) || x >= x || x > x;
+    print r, "\n"; // true
+
+    if !(x as bv5) != 23 {
+      print "one's complement: ", !x, " ", !y, " ", !z, " "; // 24 3989525554 5
+      print !(5 as bv7), " ", !(5 as bv3), " ", !(5 as bv8), "\n"; // 122 2 250
+    }
+    if -(x as bv5) != 23 {
+      print "two's complement: ", -x, " ", -y, " ", -z, " "; // 25 3989525555 6
+      print -(5 as bv7), " ", -(5 as bv3), " ", -(5 as bv8), "\n"; // 123 3 251
+    }
+
+    print "== bv: ", x == x, " ", y == y, " ", (5 as bv5) == (5 as BV) as bv5, " ", (4 as bv325) == (4 as bv325), "\n"; // true true true true
+    print "== int: ", 5 == 5, " ", (5 as int32) == (5 as BV) as int32, " ", (5 as int32) == (5 as int32), "\n"; // true true true
+    print "== real: ", 5.0 == 5.0, " ", (5.0 as MyReal) == (5.0 as MyReal), "\n"; // true true
+    print "!= bv: ", x != x, " ", y != y, " ", (5 as bv5) != (5 as BV) as bv5, " ", (4 as bv325) != (4 as bv325), "\n"; // false false false false
+    print "!= int: ", 5 != 5, " ", (5 as int32) != (5 as BV) as int32, " ", (5 as int32) != (5 as int32), "\n"; // false false false
+    print "!= real: ", 5.0 != 5.0, " ", (5.0 as MyReal) != (5.0 as MyReal), "\n"; // false false
+    print "<= bv: ", x <= x, " ", y <= y, " ", (5 as bv5) <= (5 as BV) as bv5, " ", (4 as bv325) <= (4 as bv325), "\n"; // true true true true
+    print "<= int: ", 5 <= 5, " ", (5 as int32) <= (5 as BV) as int32, " ", (5 as int32) <= (5 as int32), "\n"; // true true true
+    print "<= real: ", 5.0 <= 5.0, " ", (5.0 as MyReal) <= (5.0 as MyReal), "\n"; // true true
+
+    var c0, c1 := new MyClass, new MyClass;
+    var col0, col1, col2 := Blue, Yellow, Yellow;
+    print "== class: ", c0 == c1, " ", c0 == c0, " / "; // false true /
+    print (c0 as RefTrait) == (c1 as RefTrait), " ", (c0 as RefTrait) == (c0 as RefTrait), " / "; // false true /
+    print (c0 as object) == (c1 as object), " ", (c0 as object) == (c0 as object), " ", (c0 as object) != (c0 as object), "\n"; // false true false
+    print "== datatype: ", col0 == col1, " ", col1 == col2, " ", col2 == col2, " ", col1 != col2, "\n"; // false true true false
+  }
+
+  method Overflows()
+  {
+// SOON or never:
+//    print (18 as bv5) + 19, " ", (18 as bv5) - 19, " ", (18 as bv5) * 19, "\n"; // 5 31 22 // TODO: Go complains about the overflow here
+    var x: BV := 18;
+    var x' := x + 1;
+    print x + x', " ", x - x', " ", x * x', "\n"; // 5 31 22
+
+// SOON or never:
+//    print (0x8000_0002 as bv32) + 0x8000_0003, " "; // 5
+//    print (0x8000_0002 as bv32) - 0x8000_0003, " "; // 4294967295
+//    print (0x8000_0002 as bv32) * 0x8000_0003, "\n"; // 2147483654
+    var w: Word := 0x8000_0002;
+    var w' := w + 1;
+    print w + w', " ", w - w', " ", w * w', "\n"; // 5 4294967295 2147483654
+  }
+
+  method Shift(x: BV, y: Word, b: bv32, i: int) returns (s: BV)
+    requires 0 <= y < 5 && 0 <= b < 5 && 0 <= i < 5
+  {
+    var si: bv5 := (18 as bv5) << 1;
+    print si, " "; // 4
+    s := x << y;
+    print s, " "; // 4
+    s := x >> b;
+    print s, " "; // 4
+    s := x << i;
+    print s, "\n"; // 16
+  }
+  
+  method Rotate(x: BV, i: int, b: bv32, j: int32) returns (s: BV, a: bv5)
+    requires 0 <= b < 5 && 0 <= i < 5 && 0 <= j < 5
+  {
+    a := x.RotateLeft(i);
+    print a, " "; // 10
+    
+    a := x.RotateRight(b as int);
+    print a, " "; // 20
+
+    a := x.RotateRight(j as nat);
+    print a, " "; // 10
+    expect a == 10;
+    s := x.RotateRight(j as nat) as BV;
+    print s, "\n"; // 10
+  }
+
+  method BvZero(b: bv0) {
+    var c: bv0 := *;
+
+    print b + c, b - c, b * c, " ", !b, " ", -b, "\n"; // 000 0 0
+    print b == c, " ", b != c, " ", b <= c, " ", b < c, " ", b >= c, " ", b > c, "\n"; // true false true false true false
+    print b & c, b | c, b ^ c, " ", b << c, b << 0, b << 0 as int32, " ", b >> c, b >> 0, b >> 0 as int32, "\n"; // 000 000 000
+    print b.RotateLeft(0), " ", b.RotateRight(0), " -- ", 0 as bv0, b as int, 0 as int32 as bv0, "\n"; // 0 0 -- 000
+  }
+
+  method TestsAndConversions() returns (x: BV, y: Word, z: Big, a: bv5, b: bv32, c: bv1024, i: int, j: int32, r: bool) {
+    x := 10;
+    x := x;
+  
+    r := y is Word;
+
+    x := 10 as BV;
+    x := x as BV;
+    x := (if y < 20 then y else 2) as BV;
+    print x, " "; // 0
+    if a != 23 {
+      x := a as BV;
+    }
+
+    b := 25;
+    x := ((b & 0xF) * 2) as BV;
+    print x, " "; // 18
+    print (x as int as bv5) == x as bv5, "\n"; // true
+
+    if 0 <= i <= j as int < 23 {
+      x := i as BV;
+      x := j as BV;
+    }
+/* SOON
+    r := 10 is bv5;
+    r := x is bv5;
+    r := y is bv5;
+    r := z is bv5;
+    r := a is bv5;
+    r := b is bv5;
+    r := c is bv5;
+    r := i is bv5;
+    r := j is bv5;
+*/
+  }
+
+  newtype Bits = b: bv109 | Predicate(b)
+
+  predicate Predicate(x: bv109) {
+    true
+  }
+
+  method Comprehensions(aa: set<bv7>, bb: set<BV>, cc: set<Word>, dd: set<Bits>) returns (size: nat) {
+    var se0, se1, se2, se3;
+    se0 := set x | x in aa;
+    se1 := set x | x in bb;
+    se2 := set x | x in cc;
+    se3 := set x | x in dd;
+    return |se0| + |se1| + |se2| + |se3|;
   }
 }
